src/Reflection/WfReflective.v
@@ -1,0 +1,306 @@
+Require Import Coq.Arith.Arith Coq.Logic.Eqdep_dec.
+Require Import Crypto.Reflection.Syntax.
+Require Import Crypto.Util.Notations Crypto.Util.Tactics Crypto.Util.Option Crypto.Util.Sigma Crypto.Util.Prod.
+
+Inductive pointed_Prop := trivial | inject (_ : Prop).
+Definition and_pointed_Prop (x y : pointed_Prop) : pointed_Prop
+  := match x, y with
+     | trivial, trivial => trivial
+     | trivial, inject p => inject p
+     | inject p, trivial => inject p
+     | inject p, inject q => inject (p /\ q)
+     end.
+Definition to_prop (x : pointed_Prop) : Prop
+  := match x with
+     | trivial => True
+     | inject p => p
+     end.
+
+Local Infix "/\" := and_pointed_Prop : type_scope.
+
+Definition f_equal2 {A1 A2 B} (f : A1 -> A2 -> B) {x1 y1 : A1} {x2 y2 : A2} (H : x1 = y1)
+  := match H in (_ = y) return (x2 = y2 -> f x1 x2 = f y y2) with
+     | eq_refl =>
+       fun H0 : x2 = y2 =>
+         match H0 in (_ = y) return (f x1 x2 = f x1 y) with
+         | eq_refl => eq_refl
+         end
+     end.
+
+Section language.
+  Context (base_type_code : Type).
+  Context (interp_base_type : base_type_code -> Type).
+  Context (base_type_eq_semidec_transparent : forall t1 t2 : base_type_code, option (t1 = t2)).
+  Context (base_type_eq_semidec_is_dec : forall t1 t2, base_type_eq_semidec_transparent t1 t2 = None -> t1 <> t2).
+  Context (op : flat_type base_type_code -> flat_type base_type_code -> Type).
+  Context (op_beq : forall t1 tR, op t1 tR -> op t1 tR -> option pointed_Prop).
+  Context (op_beq_bl : forall t1 tR x y, match op_beq t1 tR x y with
+                                    | Some p => to_prop p
+                                    | _ => False
+                                    end -> x = y).
+  Context {var1 var2 : base_type_code -> Type}.
+
+  Local Notation eP := (fun t => var1 (fst t) * var2 (snd t))%type (only parsing).
+
+  Local Notation flat_type := (flat_type base_type_code).
+  Local Notation type := (type base_type_code).
+  Let Tbase := @Tbase base_type_code.
+  Local Coercion Tbase : base_type_code >-> flat_type.
+  Local Notation interp_type := (interp_type interp_base_type).
+  Local Notation interp_flat_type := (interp_flat_type_gen interp_base_type).
+  Local Notation exprf := (@exprf base_type_code interp_base_type op).
+
+  (*Fixpoint eq_interp_flat_type (t1 t2 : flat_type)
+    : interp_flat_type t1 -> interp_flat_type t2 -> option pointed_Prop
+    := match t1, t2 return interp_flat_type t1 -> interp_flat_type t2 -> option _ with
+       | Prod A B, Prod A' B'
+         => fun x y => match @eq_interp_flat_type A A' (fst x) (fst y),
+                         @eq_interp_flat_type B B' (snd x) (snd y) with
+                   | Some p, Some q => Some (p /\ q)
+                   | _, _ => None
+                   end
+       | Prod _ _, _ => fun _ _ => None
+       | Syntax.Tbase t1, Syntax.Tbase t2
+         => fun x y => base_type_eq_and_cast t1 t2 x y (*Some (exists pf : t1 = t2, eq_rect _ interp_base_type x _ pf = y)*)
+       | Syntax.Tbase _, _ => fun _ _ => None
+       end.*)
+  Fixpoint flat_type_eq_semidec_transparent (t1 t2 : flat_type) : option (t1 = t2)
+    := match t1, t2 return option (t1 = t2) with
+       | Syntax.Tbase t1, Syntax.Tbase t2
+         => option_map (@f_equal _ _ Tbase _ _)
+                      (base_type_eq_semidec_transparent t1 t2)
+       | Syntax.Tbase _, _ => None
+       | Prod A B, Prod A' B'
+         => match flat_type_eq_semidec_transparent A A', flat_type_eq_semidec_transparent B B' with
+           | Some p, Some q => Some (f_equal2 Prod p q)
+           | _, _ => None
+           end
+       | Prod _ _, _ => None
+       end.
+  Definition op_beq' t1 tR t1' tR' (x : op t1 tR) (y : op t1' tR') : option pointed_Prop
+    := match flat_type_eq_semidec_transparent t1 t1', flat_type_eq_semidec_transparent tR tR' with
+       | Some p, Some q
+         => match p in (_ = t1'), q in (_ = tR') return op t1' tR' -> _ with
+           | eq_refl, eq_refl => fun y => op_beq _ _ x y
+           end y
+       | _, _ => None
+       end.
+
+  Definition eq_type_and_var : sigT eP -> sigT eP -> option pointed_Prop
+    := fun x y =>
+         let 'existT (t1, t2) (a, b) := x in
+         let 'existT (t1', t2') (a', b') := y in
+         match base_type_eq_semidec_transparent t1 t1', base_type_eq_semidec_transparent t2 t2' with
+         | Some p, Some q
+           => Some (inject (and (eq_rect _ var1 a _ p = a') (eq_rect _ var2 b _ q = b')))
+         | _, _ => None
+         end.
+
+
+  Definition duplicate_type (ls : list (sigT (fun t => var1 t * var2 t)%type)) : list (sigT eP)
+    := List.map (fun v => existT eP (projT1 v, projT1 v) (projT2 v)) ls.
+
+  Lemma duplicate_type_app ls ls'
+    : (duplicate_type (ls ++ ls') = duplicate_type ls ++ duplicate_type ls')%list.
+  Proof. apply List.map_app. Qed.
+  Lemma duplicate_type_length ls
+    : List.length (duplicate_type ls) = List.length ls.
+  Proof. apply List.map_length. Qed.
+  (** TODO: Clean up this proof *)
+  Lemma base_type_eq_dec : forall t1 t2 : base_type_code, {t1 = t2} + {t1 <> t2}.
+  Proof.
+    intros t1 t2; destruct (base_type_eq_semidec_transparent t1 t2) eqn:H;
+      [ left; assumption | right; auto using base_type_eq_semidec_is_dec ].
+  Qed.
+  Lemma duplicae_type_in t v ls
+    : List.In (existT _ (t, t) v) (duplicate_type ls) -> List.In (existT _ t v) ls.
+  Proof.
+    unfold duplicate_type; intro H.
+    apply List.in_map_iff in H.
+    destruct H as [ [t' ?] [? ?] ].
+    simpl in *.
+    inversion_sigma; subst.
+    match goal with H : _ |- _ => generalize (path_prod_eta H) end.
+    let x := match goal with |- ?x = _ -> _ => x end in
+    generalize (fst_path x); generalize (snd_path x); simpl.
+    intro; subst; intro H'; intros; subst.
+    assert (H' = eq_refl) by apply UIP_dec, base_type_eq_dec.
+    subst; simpl; assumption.
+  Qed.
+  Lemma duplicate_type_not_in G t t0 v (H : base_type_eq_semidec_transparent t t0 = None)
+    : ~List.In (existT _ (t, t0) v) (duplicate_type G).
+  Proof.
+    apply base_type_eq_semidec_is_dec in H.
+    clear -H.
+    intro H'.
+    induction G as [|? ? IHG]; simpl in *; try tauto.
+    destruct H'; intuition eauto; congruence.
+  Qed.
+
+  Definition preflatten_binding_list2 t1 t2 : option (forall (x : interp_flat_type_gen var1 t1) (y : interp_flat_type_gen var2 t2), list (sigT (fun t => var1 t * var2 t)%type))
+    := match flat_type_eq_semidec_transparent t1 t2 with
+       | Some p
+         => Some (fun x y
+                 => let x := eq_rect _ (interp_flat_type_gen var1) x _ p in
+                   flatten_binding_list base_type_code x y)
+       | None => None
+       end.
+  Definition flatten_binding_list2 t1 t2 : option (forall (x : interp_flat_type_gen var1 t1) (y : interp_flat_type_gen var2 t2), list (sigT eP))
+    := option_map (fun f x y => duplicate_type (f x y)) (preflatten_binding_list2 t1 t2).
+  Fixpoint natize_interp_flat_type_gen {var t} (base : nat) (v : interp_flat_type_gen var t) {struct t}
+    : nat * interp_flat_type_gen (fun t : base_type_code => nat * var t)%type t
+    := match t return interp_flat_type_gen var t -> nat * interp_flat_type_gen _ t with
+       | Prod A B => fun v => let ret := @natize_interp_flat_type_gen _ B base (snd v) in
+                          let base := fst ret in
+                          let b := snd ret in
+                          let ret := @natize_interp_flat_type_gen _ A base (fst v) in
+                          let base := fst ret in
+                          let a := snd ret in
+                          (base, (a, b))
+       | Syntax.Tbase t => fun v => (S base, (base, v))
+       end v.
+  Lemma length_natize_interp_flat_type_gen1 {t} (base : nat) (v1 : interp_flat_type_gen var1 t) (v2 : interp_flat_type_gen var2 t)
+    : fst (natize_interp_flat_type_gen base v1) = length (flatten_binding_list base_type_code v1 v2) + base.
+  Proof.
+    revert base; induction t; simpl; [ reflexivity | ].
+    intros; rewrite List.app_length, <- plus_assoc.
+    rewrite_hyp <- ?*; reflexivity.
+  Qed.
+  Lemma length_natize_interp_flat_type_gen2 {t} (base : nat) (v1 : interp_flat_type_gen var1 t) (v2 : interp_flat_type_gen var2 t)
+    : fst (natize_interp_flat_type_gen base v2) = length (flatten_binding_list base_type_code v1 v2) + base.
+  Proof.
+    revert base; induction t; simpl; [ reflexivity | ].
+    intros; rewrite List.app_length, <- plus_assoc.
+    rewrite_hyp <- ?*; reflexivity.
+  Qed.
+
+  Fixpoint unnatize_exprf {var t} (base : nat) (e : @exprf (fun t => nat * var t)%type t) : @exprf var t
+    := match e in @Syntax.exprf _ _ _ _ t return exprf t with
+       | Const _ x => Const x
+       | Var _ x => Var (snd x)
+       | Op _ _ op args => Op op (@unnatize_exprf _ _ base args)
+       | Let _ ex _ eC => Let (@unnatize_exprf _ _ base ex) (fun x => let v := natize_interp_flat_type_gen base x in
+                                                                  @unnatize_exprf _ _ (fst v) (eC (snd v)))
+       | Pair _ x _ y => Pair (@unnatize_exprf _ _ base x) (@unnatize_exprf _ _ base y)
+       end.
+
+  Fixpoint reflect_wffT (G : list (sigT (fun t => var1 (fst t) * var2 (snd t))%type))
+           {t1 t2 : flat_type}
+           (e1 : @exprf (fun t => nat * var1 t)%type t1) (e2 : @exprf (fun t => nat * var2 t)%type t2)
+           {struct e1}
+    : option pointed_Prop
+    := match e1, e2 return option _ with
+       | Const t0 x, Const t1 y
+         => match flat_type_eq_semidec_transparent t0 t1 with
+           | Some p => Some (inject (eq_rect _ interp_flat_type x _ p = y))
+           | None => None
+           end
+       | Const _ _, _ => None
+       | Var t0 x, Var t1 y
+         => match Nat.eqb (fst x) (fst y), List.nth_error G (List.length G - S (fst x)) with
+           | true, Some v => eq_type_and_var v (existT _ (t0, t1) (snd x, snd y))
+           | _, _ => None
+           end
+       | Var _ _, _ => None
+       | Op t1 tR op args, Op t1' tR' op' args'
+         => match @reflect_wffT G t1 t1' args args', op_beq' t1 tR t1' tR' op op' with
+           | Some p, Some q => Some (p /\ q)
+           | _, _ => None
+           end
+       | Op _ _ _ _, _ => None
+       | Let tx ex tC eC, Let tx' ex' tC' eC'
+         => match @reflect_wffT G tx tx' ex ex', @flatten_binding_list2 tx tx', flat_type_eq_semidec_transparent tC tC' with
+           | Some p, Some G0, Some _
+             => Some (p /\ inject (forall (x : interp_flat_type_gen var1 tx) (x' : interp_flat_type_gen var2 tx'),
+                                    match @reflect_wffT (G0 x x' ++ G)%list _ _
+                                                       (eC (snd (natize_interp_flat_type_gen (List.length G) x)))
+                                                       (eC' (snd (natize_interp_flat_type_gen (List.length G) x'))) with
+                                    | Some p => to_prop p
+                                    | None => False
+                                    end))
+           | _, _, _ => None
+           end
+       | Let _ _ _ _, _ => None
+       | Pair tx ex ty ey, Pair tx' ex' ty' ey'
+         => match @reflect_wffT G tx tx' ex ex', @reflect_wffT G ty ty' ey ey' with
+           | Some p, Some q => Some (p /\ q)
+           | _, _ => None
+           end
+       | Pair _ _ _ _, _ => None
+       end.
+
+  Local Ltac handle_op_beq_correct :=
+    repeat match goal with
+           | [ H : op_beq ?t1 ?tR ?x ?y = _ |- _ ]
+             => let H' := fresh in
+               pose proof (op_beq_bl t1 tR x y) as H'; rewrite H in H'; clear H
+           end.
+  Local Ltac t_step :=
+    match goal with
+    | _ => progress unfold eq_type_and_var, op_beq', flatten_binding_list2, preflatten_binding_list2, option_map in *
+    | _ => progress simpl in *
+    | _ => progress break_match
+    | _ => progress subst
+    | _ => progress inversion_option
+    | _ => congruence
+    | _ => tauto
+    | _ => progress intros
+    | _ => progress handle_op_beq_correct
+    | _ => progress specialize_by tauto
+    | [ H : forall x x', _ |- wff _ _ _ (flatten_binding_list _ ?x1 ?x2 ++ _)%list _ _ ]
+      => specialize (H x1 x2)
+    | [ H : and _ _ |- _ ] => destruct H
+    | [ H : context[duplicate_type (_ ++ _)%list] |- _ ]
+      => rewrite duplicate_type_app in H
+    | [ H : context[List.length (duplicate_type _)] |- _ ]
+      => rewrite duplicate_type_length in H
+    | [ H : context[List.length (_ ++ _)%list] |- _ ]
+      => rewrite List.app_length in H
+    | [ |- wff _ _ _ _ (unnatize_exprf (fst _) _) (unnatize_exprf (fst _) _) ]
+      => erewrite length_natize_interp_flat_type_gen1, length_natize_interp_flat_type_gen2; eassumption
+    | [ H : base_type_eq_semidec_transparent _ _ = None |- False ] => eapply duplicate_type_not_in; eassumption
+    | [ H : List.nth_error _ _ = Some _ |- _ ] => apply List.nth_error_In in H
+    | [ H : List.In _ (duplicate_type _) |- _ ] => apply duplicae_type_in in H
+    | [ H : context[match _ with _ => _ end] |- _ ] => revert H; progress break_match
+    | [ H : inject _ = inject _ |- _ ] => inversion H; clear H
+    | [ |- wff _ _ _ _ _ _ ] => constructor
+    | _ => progress unfold and_pointed_Prop in *
+    end.
+  Local Ltac t := repeat t_step.
+  Fixpoint reflect_wff (G : list (sigT (fun t => var1 t * var2 t)%type))
+           {t1 t2 : flat_type}
+           (e1 : @exprf (fun t => nat * var1 t)%type t1) (e2 : @exprf (fun t => nat * var2 t)%type t2)
+           {struct e1}
+    : match reflect_wffT (duplicate_type G) e1 e2 with
+      | Some p => to_prop p
+      | None => False
+      end
+      -> match flat_type_eq_semidec_transparent t1 t2 with
+        | Some p => @wff base_type_code interp_base_type op var1 var2 G t2 (eq_rect _ exprf (unnatize_exprf (List.length G) e1) _ p) (unnatize_exprf (List.length G) e2)
+        | None => False
+        end.
+  Proof.
+    destruct e1 as [ | | ? ? ? args | tx ex tC eC | ? ex ? ey ],
+                   e2 as [ | | ? ? ? args' | tx' ex' tC' eC' | ? ex' ? ey' ]; simpl; try solve [ intros [] ];
+      [ clear reflect_wff
+      | clear reflect_wff
+      | specialize (reflect_wff G _ _ args args')
+      | pose proof (reflect_wff G _ _ ex ex');
+        pose proof (fun x x'
+                    => match preflatten_binding_list2 tx tx' as v return match v with Some _ => _ | None => True end with
+                      | Some G0
+                        => reflect_wff
+                            (G0 x x' ++ G)%list _ _
+                            (eC (snd (natize_interp_flat_type_gen (length (duplicate_type G)) x)))
+                            (eC' (snd (natize_interp_flat_type_gen (length (duplicate_type G)) x')))
+                      | None => I
+                      end);
+        clear reflect_wff
+      | pose proof (reflect_wff G _ _ ex ex'); pose proof (reflect_wff G _ _ ey ey'); clear reflect_wff ].
+    { t. }
+    { t. }
+    { t. }
+    { t. }
+    { t. }
+  Qed.
+End language.
